AwsCryptographyPrimitives/test/TestRSA.dfy
@@ -8,10 +8,48 @@ module TestAwsCryptographyPrimitivesRSA {
   import Aws.Cryptography.Primitives
   import opened Wrappers
   import opened StandardLibrary.UInt
+  import UTF8
+
+  const RSA_PUBLIC_2048 := "-----BEGIN PUBLIC KEY-----\n"
+    + "MIIBIjANBgkqhkiG9w0BAQEFAAOCAQ8AMIIBCgKCAQEAqBvECLsPdF1J5DOkaA1n\n"
+    + "UrGwNT9ard3KSMaPypla/5Jhz0veCz1OSjnx35+FE3q7omHQBmKRs6XDkj4tJ5vh\n"
+    + "1baw2yzgIAqW9lOXK64GiYy0maH2NfRxGbj5LhVq5T4YOkKh9D3GFbfT9/NpcsOZ\n"
+    + "M2HDX8Z+M0HM3XymtcfpHk5o6QF1lbBW+rDJEcYhPN0obBufCXaasgsBRP5Ei2b5\n"
+    + "18xpy9M19By1yuC9mlNcpE5v5A8fq/qLLT4s34/6dnVxKX6gIoWDzDrUNrnPe0p5\n"
+    + "pqZ1SHalrELMf/liXPrf94+0cF8g1fYVGGo+MZsG5/HRngLiskP25w5smMT51U1y\n"
+    + "gQIDAQAB\n"
+    + "-----END PUBLIC KEY-----";
+
+  const RSA_PUBLIC_3072 := "-----BEGIN PUBLIC KEY-----\n"
+    + "MIIBojANBgkqhkiG9w0BAQEFAAOCAY8AMIIBigKCAYEAnrUonUAKKpZE+LbQfq6I\n"
+    + "gAR//GNnT7L6P3LCboXu44StJtvVyAmHZXPgdkxxT1EKLFx+Tys3B7jhgno9cs67\n"
+    + "Scf0pLjJAmXOVHa6881oxi5zeP0e6+KzOPugg3C+EknS2PSHTLsdTrkgZU+oUjde\n"
+    + "AgRSgmWrp8aMM1WpoLmNcWC/Pi0mSziVnIzE3WhkZ2Ccetz/viRL60VHlTwNQPVa\n"
+    + "7fqbcSqBxm/VjDzYvDwzmU+4GNEs5hrA2IFDxxsYZAU8HdASQM18A8W7n0Okaa4e\n"
+    + "c4svyKVFkncbNCqetynLU0A5ny7I5WVXV7DNi2VMjD/mZsEt8IrwfuWSMKuIPxs/\n"
+    + "Nb/4Psr7ZvbKSlaMwEpyReHvYYqM7dd6A4Y9FirnrpAPaqlfm8UFtHKQvUckxRoR\n"
+    + "05kzNN2jIRJtMwGpn+40tiei7eBGMmIn41/dnkM7GOJau4BarSJMiREK1yH9hh1C\n"
+    + "GbrQu6i0F9G0uBDITen9/uPX9cxK5pNHAxeWzr2UP1UzAgMBAAE=\n"
+    + "-----END PUBLIC KEY-----";
+
+  const RSA_PUBLIC_4096 := "-----BEGIN PUBLIC KEY-----\n"
+    + "MIICIjANBgkqhkiG9w0BAQEFAAOCAg8AMIICCgKCAgEAs86OIUN9RbdEdyQb2tGQ\n"
+    + "miDmmeJaYKanLB0lfWiuO85kJK8edZyLkHIzps81qwgVSzbMCBB7QGcMyPbb3wbE\n"
+    + "B4EJ32v3cuMVUs6sOvOYV4g1c1Hi1WVqnCeH+3RSFBfb7RL7SvSUmilX2tNV6uZy\n"
+    + "BmMSGBJ/IMzxoHjKSFn6r1ttwov8X5DmNTyIp4qG3qyL1qhpla1bUE5Nb6uMHI2v\n"
+    + "qMM+8zSPcRN40CfaQATxevNs/69++XJ+5L1nKU9fMwust1GEbtJ6cIBwAuqlyMm9\n"
+    + "CnZ+tn56FEVPrUrsQX35QRNjbi0jjKI8ItkdyJ5fLixCjJ20tCo5jeL5KJ32Rjuw\n"
+    + "BlB2KQrgdw5VEMrMlTJz9oozUv8GFzjtS4kx+tAsWhji5s0jry4QFYG01Q4ezVPb\n"
+    + "TYdxg1Yz265EyLmF0+/ZQtO1kQc7tXHD5Gzzwyqot/UdJwlXStUGB2yEe62HQ2LT\n"
+    + "9Ly3V7rUDJzO44zuFVjqchRPYWNdiYl8BVP/ak2bMtcowk06T9bo1tRf4HJWfpIM\n"
+    + "GF27MXqykKHxcmOb0UfGIfI0eUtkid4gJdCxhidiILj6SHpEr+oa/Oogz01rVCdm\n"
+    + "mbWmgFxmiKse8NXNQR+7qhMYX5GgdeSbp/Lg24HF9mvnd0S2wHkC86lGyQtvzrsd\n"
+    + "DdUJZ2jqiKvMLdMKNFHFGGUCAwEAAQ==\n"
+    + "-----END PUBLIC KEY-----";
 
   method {:test} RSAEncryptTests() {
     var client :- expect Primitives.AtomicPrimitives();
-    var keys := client.GenerateRSAKeyPair(input := Primitives.Types.GenerateRSAKeyPairInput(strength := 2048 as Primitives.Types.RSAStrengthBits));
+    var keys := client.GenerateRSAKeyPair(input := Primitives.Types.GenerateRSAKeyPairInput(lengthBits := 2048 as Primitives.Types.RSAModulusLengthBits));
     expect keys.Success?;
 
     BasicRSAEncryptTest(
@@ -23,6 +61,29 @@ module TestAwsCryptographyPrimitivesRSA {
       ),
       keys.value
     );
+  }
+  
+  method {:test} GetRSAKeyModulusLength() {
+    var client :- expect Primitives.AtomicPrimitives();
+
+    // 2048
+
+    var publicKey2048 :- expect UTF8.Encode(RSA_PUBLIC_2048);
+    var length2048 :- expect client.GetRSAKeyModulusLength(
+      Primitives.Types.GetRSAKeyModulusLengthInput(publicKey := publicKey2048));
+    expect length2048.length == 2048;
+
+    // 3072
+    var publicKey3072 :- expect UTF8.Encode(RSA_PUBLIC_3072);
+    var length3072 :- expect client.GetRSAKeyModulusLength(
+      Primitives.Types.GetRSAKeyModulusLengthInput(publicKey := publicKey3072));
+    expect length3072.length == 3072;
+
+    // 4096
+    var publicKey4096 :- expect UTF8.Encode(RSA_PUBLIC_4096);
+    var length4096 :- expect client.GetRSAKeyModulusLength(
+      Primitives.Types.GetRSAKeyModulusLengthInput(publicKey := publicKey4096));
+    expect length4096.length == 4096;
   }
 
   method BasicRSADecryptTests(
